
\chapter{Multi-step Methods}
Methods using the approximation at more than one previous point to determine the
approx at the next point are called multi-step methods.
\begin{definition}
An m-step multi-step method for solving the \addtoindex{Initial Value Problem}
\[y^{'} = f(t,y) \ \ a\leq t \leq b \ \ y(a) =\alpha\]
is on whose difference equation for finding the approximation $w_{i+1}$ at the
mesh points $t_{i+1}$ can be represented by the following equation, when m is
an integer greater than 1,
\[w_{i+1}  =  a_{m-1}w_i +a_{m-2}w_{i-1} + ... + a_{0}w_{i+1-m}\]
\begin{equation}
\label{multi}
+h[b_{m}f(t_{i+1},w_{i+1}) + b_{m-1}f(t_{i},w_{i}) +...+ b_{0}f(t_{i+1-m},w_{i+1-m}) ]
\end{equation}
for $i=m-1,m,...,N-1$ where $h=\frac{b-a}{N}$ the $a_0,a_1,...,a_m-1$ and $b_0,b_1,...,b_m$
are constants, and the starting values 
\[ w_0=\alpha, \ \ w_1=\alpha_1, \ \ w_2=\alpha_2, \ ... \ w_{m-1}=\alpha_{m-1} \] 
are specified.\\
When $b_m=0$ the method is called \textbf{explicit} or open since (\ref{multi}) then gives
$w_{i+1}$ explicitly in terms of previously determined approximations.

When $b_m\not=0$ the method is called \textbf{implicit} or closed since $w_{i+1}$ occurs on both sides of (\ref{multi}). 
$\diamond$
\end{definition}
\begin{example}
Fourth order \addtoindex{Adams-Bashforth}
\[w_0=\alpha \ \ \ w_1=\alpha_1 \ \ \ w_2 = \alpha_2 \ \ \ w_3 = \alpha_3 \]

\begin{eqnarray*}
w_{i+1} &=& w_i +  \frac{h}{24}[55f(t_i,w_i)-59f(t_{i-1},w_{i-1})\\
& & +  37f(t_{i-2},w_{i-2})-9f(t_{i-3},w_{i-3})]
\end{eqnarray*}

For each $i=3,4,...,N-1$ define an explicit four step method known as the fourth
order \addtoindex{Adams-Bashforth} technique.\\
The equation
\[w_0=\alpha \ \ \ w_1=\alpha_1 \ \ \ w_2 = \alpha_2  \]
\begin{eqnarray*}w_{i+1} &=& w_i + \frac{h}{24}[9f(t_{i+1},w_{i+1})+19f(t_{i},w_{i})\\
& &-5f(t_{i-1},w_{i-1})+f(t_{i-2},w_{i-2})]\end{eqnarray*}
For each $i=2,4,...,N-1$ define an implicit three step method known as the fourth
order \addtoindex{Adams-Moulton} technique.
\end{example}
\textbf{For the previous methods we need to generate $\alpha_1,\alpha_2$ and $\alpha_3$ by using a one step method.}
\section{Derivation of a explicit multistep method}


\subsection{General Derivation of a explicit method Adams-Bashforth}

\[y(t_{i+1})-y(t_{i}) = \int_{t_i}^{t_{i+1}} y^{'}(t) dt=\int_{t_i}^{t_{i+1}} f(t,y(t)) dt \]
Consequently
\[y(t_{i+1})=y(t_{i}) + \int_{t_i}^{t_{i+1}} f(t,y(t)) dt\]
Since we cannot  integrate $f(t,y(t))$ without knowing $y(t)$ the solution to the problem
we instead integrate an interpolating poly. $P(t)$ to $f(t,y(t))$ that is determined
by some of the previous obtained data points $(t_0,w_0), (t_1,w_1),...,(t_i,w_i)$.
When we assume in addition that $y(t_i)\approx w_i$
\[y(t_{i+1})\approx w_{i} + \int_{t_i}^{t_{i+1}} P(t) dt\]
We use Newton back-substitution to derive an \addtoindex{Adams-Bashforth} explicit m-step technique,
we form the backward difference poly $P_{m-1}(t)$ through $(t_i,f(t_i)),(t_{i-1},f(t_{i-1})),...,(t_{i+1-m},f(t_{i+1-m}))$
\begin{equation}
    f(t,y(t))=P_{m-1}(t)+f^{m}(\xi,y(\xi))\frac{(t-t_i)...(t-t_{i+1-m})}{m!}
\end{equation}

\begin{equation}
    P_{m-1}(t)=\Sigma_{j=1}^{m} L_{m-1,j}(t)\nabla^j f(t_{i+1-j},y(t_{i+1-j}))\end{equation}
where \[\nabla f(t_i,y(t_i)) = f(t_i,y(t_i))-f(t_{i-1},y(t_{i-1})),\]
\[\nabla^2 f(t_i,y(t_i)) = \nabla f(t_i,y(t_i))-\nabla f(t_{i-1},y(t_{i-1}))\]
\[=f(t_i,y(t_i))-2f(t_{i-1},y(t_{i-1}))+f(t_{i-2},y(t_{i-2})).\]
\subsubsection*{Derivation of a explicit two-step method Adams Bashforth}
To derive two step \addtoindex{Adams-Bashforth} technique
\begin{eqnarray*}
\int_{t_i}^{t_{i+1}} f(t,y)dt &= &\int_{t_i}^{t_{i+1}}[f(t_i,y(t_i))+\frac{(t-t_i)}{h}\nabla f(t_i,y(t_i))+error]dt \\
y_{i+1}-y_i &= &[tf(t_i,y(t_i))+\frac{t(\frac{t}{2}-t_i)}{h}\nabla f(t_i,y(t_i))]_{t_i}^{t_{i+1}}+Error \\
y_{i+1}&=&y(t_i)+ (t_{i+1}-t_i)f(t_i,y(t_i))\\
& & +\frac{\frac{t_{i+1}}{2}-t_{i+1}t_i+\frac{t_i^2}{2}-t_i^2}{h}\nabla(f(t_i,y(t_i))+Error\\
&=&y(t_i)+ hf(t_i,y(t_i))\\
& & +\frac{(t_{i+1}-t_i)^2}{2h}(f(t_i,y(t_i))-f(t_{i-1},y(t_{i-1})))+Error\\
&=&y(t_i)+ hf(t_i,y(t_i))\\
& & +\frac{1}{2}(f(t_i,y(t_i))-f(t_{i-1},y(t_{i-1})))+Error\\
&=&y(t_i)+ \frac{h}{2}[3f(t_i,y(t_i))-f(t_{i-1},y(t_{i-1}))+Error]
\end{eqnarray*}
The two step \addtoindex{Adams-Bashforth} is $w_0=\alpha_0$ and $w_1=\alpha_1$ with
\[w_{i+1}=w_i+\frac{h}{2}[3w_{i}-w_{i-1}] \ \ \ for \ \ i=1,..,N-1 \]

The local truncation error is
\[\tau_{i+1}(h)=\frac{y(t_i+1)-y(t_i)}{h}-\frac{1}{2}[3f(t_i,y(t_i))-f(t_{i-1},y(t_{i-1})) ]  \]
\[\tau_{i+1}(h)=\frac{Error}{h}\]

\begin{eqnarray*}
Error &= &\int_{t_i}^{t_{i+1}} \frac{(t-t_i)(t-t_{i-1})}{2!} f^2(\mu_i,y(\mu_i))]dt \\
&=&\frac{5}{12}h^3f^2(\mu_i,y(\mu_i))\\
\end{eqnarray*}
\[\tau_{i+1}(h)=\frac{\frac{5}{12}h^3f^2(\mu_i,y(\mu_i))}{h}\]
The local truncation error for the two step Adams-Bashforth methods is of order 2
\[\tau_{i+1}(h)=O(h^2)\]

\subsection*{General Derivation of a explicit method Adams-Bashforth (cont.)}


\begin{definition}
The Lagrange polynomial $L_{m-1,j}(t)$ has a degree of $m-1$ and is associated with the interpolation point $t_j$ in the sense
\[
L_{m-1,j}(t)=\left\{
                \begin{array}{ll}
                  1 & i=j\\
                  0 & i\neq j
                      \end{array}
              \right.
\]
\begin{equation}
    L_{m-1,j}(t)=\frac{(t-t_0)...(t-t_{m-1})}{(t_j-t_0)...(t_j-t_{m-1})}=\prod_{k=0, k \neq j}^{m-1} \frac{t-t_k}{t_j-t_k}
\end{equation}

\end{definition}

Introducing the variable $t=t_k+sh$ with $dt=hds$ into $L_{m-1}(t)$ 
\begin{equation}
    L_{m-1,j}(t)=\prod_{k=0, k \neq j}^{m-1}  \frac{t_i+sh-t_k}{(i+1)h}= (-1)^{(m-1)} \left(\begin{array}{c}-s \\ (m-1) \end{array}\right)
\end{equation}


\begin{eqnarray*}
\int_{t_i}^{t_{i+1}} f(t,y(t)) dt=& \int_{t_i}^{t_{i+1}}\sum_{k=0}^{m-1}\left(\begin{array}{c}-s \\ k \end{array}\right) \nabla^k f(t_i,y(t_i))dt\\
& +\int_{t_i}^{t_{i+1}}f^{m}(\xi,y(\xi))\frac{(t-t_i)...(t-t_{i+1-m})}{m!}dt \\
 =&\sum_{k=0}^{m-1}\nabla^k  f(t_i,y(t_i))h(-1)^k\int_{0}^{1}\left(\begin{array}{c}-s \\ k \end{array}\right)ds\\
 & +\frac{h^{m+1}}{m!}\int_{0}^{1}s(s+1)...(s+m-1)f^{m}(\xi,y(\xi))ds
 \end{eqnarray*}
The integrals $(-1)^k\int_{0}^{1}\left(\begin{array}{c}-s \\ k \end{array}\right)ds$ for various values of k are computed as such,
\begin{example}
Example $k=2$
\begin{eqnarray*}
(-1)^2\int_{0}^{1}\left(\begin{array}{c}-s \\ 2 \end{array}\right)ds
&=& \int_{0}^{1} \frac{-s(-s-1)}{1.2}ds\\
&=& \frac{1}{2} \int_{0}^{1} s^2+s ds\\
&=& \frac{1}{2} \left[ \frac{s^3}{3}+\frac{s^2}{2}\right]^{1}_{0}=\frac{5}{12}
\end{eqnarray*}
\end{example}

\begin{table}[H]
\begin{center}
\caption{Table of Adams-Bashforth coefficients}
\begin{tabular}{l|c|c|c|c|c|r}
\hline
k&0&1&2&3&4&...\\
\hline
$(-1)^k\int_{0}^{1}\left(\begin{array}{c}-s \\ k \end{array}\right)ds$& 1 & $\frac{1}{2}$ &$ \frac{5}{12}$ & $\frac{3}{8}$ & .&..
\end{tabular}
\end{center}
\end{table}
As a consequence
\[ \int_{t_i}^{t_{i+1}} f(t,y(t)) dt= h\left[ f(t_i,y(t_i))+\frac{1}{2}\nabla f(t_i,y(t_i))+\frac{5}{12}\nabla^{2} f(t_i,y(t_i))+...\right]\]
\[
+\frac{h^{m+1}}{m!}\int_{0}^{1}s(s+1)...(s+m-1)f^{m}(\xi,y(\xi))ds
\]
Since $s(s+1)...(s+m-1)$ does not change sign on $[0,1]$ it can be stated that for some $\mu_i$ where $t_{i+1-m} < \mu_i < t_{i+1}$ the error term becomes
\[
\frac{h^{m+1}}{m!}\int_{0}^{1}s(s+1)...(s+m-1)f^{m}(\xi,y(\xi))ds
\]
\[
\frac{h^{m+1}}{m!}f^{m}(\mu,y(\mu))\int_{0}^{1}s(s+1)...(s+m-1)ds
\]
Since $y(t_{i+1})-y(t_i)=\int_{t_{i}}^{t_{i+1}}f(s,y(s))ds $ this can be written as
\[y(t_{i+1})=y(t_{i})+h\left[ f(t_i,y(t_i))+\frac{1}{2}\nabla f(t_i,y(t_i))+\frac{5}{12}\nabla^{2} f(t_i,y(t_i))+...\right]\]

\begin{example}
To derive the two step Adams-Bashforth method
\begin{eqnarray*}
y(t_{i+1}) &\approx &y(t_i)+ h[f(t_i,y(t_i))+\frac{1}{2}(\nabla f(t_i,y(t_i)))] \\
&=&y(t_i)+ h[f(t_i,y(t_i))\\
& &+\frac{1}{2}(f(t_i,y(t_i))-f(t_{i-1},y(t_{i-1})))]\\
&=&y(t_i)+ \frac{h}{2}[3f(t_i,y(t_i))-f(t_{i-1},y(t_{i-1}))]
\end{eqnarray*}
The two step \addtoindex{Adams-Bashforth} is $w_0=\alpha_0$ and $w_1=\alpha_1$ with
\[w_{i+1}=w_i+\frac{h}{2}[3w_{i}-w_{i-1}] \ \ \ for \ \ i=1,..,N-1 \]
\end{example}

\begin{definition}
If $y(t)$ is a solution of the \addtoindex{Initial Value Problem}
\[y^{'}=f(t,y),\ \ \ a\leq t \leq b \ \ y(a)=\alpha \]
and
\[ w_{i+1} = a_{m-1}w_i +a_{m-2}w_{i-1} + ... + a_{0}w_{i+1-m}\]
\[
+h[b_{m}f(t_{i+1},w_{i+1}) + b_{m-1}f(t_{i},w_{i}) +...+ b_{0}f(t_{i+1-m},w_{i+1-m}) ]
\]
is the (i+1)th step in a multi-step method, the local truncation error at this step is
\[\tau_{i+1}(h)=\frac{y(t_{i+1})-
a_{m-1}y(t_i)  - ... - a_{0}y(t_{i+1-m})}{h}\]
\[
-[b_{m}f(t_{i+1},y(t_{i+1})) + b_{m-1}f(t_{i},y(t_{i})) +...+ b_{0}f(t_{i+1-m},y(t_{i+1-m})) ]
\]
for each $i=m-1,...,N-1$.
\end{definition}
\begin{example}
Truncation error for the two step \addtoindex{Adams-Bashforth} method is
\[h^3f^2(\mu_i,y(\mu_i))(-1)^2\int_{0}^1\left(\begin{array}{c}-s \\ 2 \end{array}\right)ds=\frac{5h^3}{12}f^2(\mu_i,y(\mu_i)) \]
using the fact that $f^2(\mu_i,y(\mu_i))=y^3(\mu_i)$
\[\tau_{i+1}(h) = \frac{y(t_{i+1})-y(t_i)}{h}-\frac{1}{2}[3f(t_i,y(t_i))-f(t_{i-1},y(t_{i-1}))] \]
\[=\frac{1}{h}\left[\frac{5h^3}{12}f^2(\mu_i,y(\mu_i))\right] =
\frac{5}{12}h^2 y^3(\mu_i)\]
\end{example}

\subsection{Adams-Bashforth three step method}
\[ w_0=\alpha \ \ w_1=\alpha_1 \ \ w_2 = \alpha_2 \]
\[w_{i+1} = w_{i}+\frac{h}{12}[23f(t_i,w_i) -16 f(t_{i-1},w_{i-1})+5f(t_{i-2},w_{i-2})] \]
where i=2,3,...,N-1\\
The local truncation error is of order 3 
\[\tau_{i+1}(h) =\frac{3}{8}h^3 y^4(\mu_i)\]
$\mu_i \in (t_{i-2},t_{i+1})$


\subsection{Adams-Bashforth four step method}
\[ w_0=\alpha, \ \ w_1=\alpha_1, \ \ w_2 = \alpha_2, \ \ w_3=\alpha_3, \]
\[w_{i+1} = w_{i}+\frac{h}{24}[55f(t_i,w_i) -59 f(t_{i-1},w_{i-1})+37f(t_{i-2},w_{i-2}) -9 f(t_{i-3},w_{i-3})], \]
where $i=3,...,N-1.$\\
The local truncation error is of order 4 
\[\tau_{i+1}(h) =\frac{251}{720}h^4 y^5(\mu_i),\]
$\mu_i \in (t_{i-3},t_{i+1}).$

\begin{example}
\[ y^{'}=y-t^2+1, \ \ \ 0 \leq t \leq 2, \ \ \ y(0)=0.5, \]
\addtoindex{Adams-Bashforth} two step
$w_0=\alpha_0$ and $w_1=\alpha_1$ with
\[w_{i+1}=w_i+\frac{h}{2}[3f(t_i,w_{i})-f(t_{i-1},w_{i-1})], \ \ \ for, \ \ i=1,..,N-1, \]
truncation error \[ \tau_{i+1}(h)=\frac{5}{12}h^2 y^3(\mu_i), \ \ \ \ \ \mu_i \in (t_{i-1},t_{i+1}).\]
\begin{enumerate}
\item Calculate $\alpha_0$ and $\alpha_1$.\\
From the initial condition we have $w_0=0.5.$\\
To calculate $w_1$ we use the modified Euler method.
\begin{eqnarray*}
w_0&=&\alpha\\
\end{eqnarray*}
We only need this to calculate $w_1$
\begin{eqnarray*}
w_{1} &=& w_0 +\frac{h}{2}[f(t_0,w_0)+f(t_{1},w_0+hf(t_0,w_0))]. 
\end{eqnarray*}
\begin{eqnarray*}
w_0&=&0.5\\
w_{1} &=& w_0 +\frac{h}{2}[f(t_0,w_0)+f(t_{1},w_0+hf(t_0,w_0))] \\
w_{1} &=& w_0 +\frac{0.2}{2}[w_0-t^2_0+1+w_0+h(w_0-t^2_0+1)-t_1^2+1] \\
 &=& 0.5 +\frac{0.2}{2}[0.5-0+1+0.5+0.2(1.5)-(0.2)^2+1] \\
 &=& 0.826
\end{eqnarray*}
we now have $\alpha_1=w_1=0.826.$
\item Calculate $w_i$ for $i=2,...N.$
\begin{eqnarray*}
w_{2}&=&w_1+\frac{h}{2}[3f(t_1,w_{1})-f(t_0,w_{0})] \\
&=&w_1+\frac{h}{2}[3(w_{1}-t_1^2+1)-(w_{0}-t_0^2+1)] \\
&=&0.826+\frac{0.2}{2}[3(0.826-0.2^2+1)-(0.5-0^2+1)] \\
&=&0.8858 \\
.\\
.\\
.\\
w_{i+1}&=&w_i+\frac{0.2}{2}[3(w_{i}-t_i^2+1)-(w_{i-1}-t_{i-1}^2+1)] 
\end{eqnarray*}
\end{enumerate}
this method can be generalised for all \addtoindex{Adams-Bashforth}.
\end{example}

\section{Derivation of the implicit multi-step method}


\subsubsection{Derivation of an implicit one-step method Adams Moulton}
To derive one step \addtoindex{Adams-Moulton} technique
\begin{eqnarray*}
\int_{t_i}^{t_{i+1}} f(t,y)dt &= &\int_{t_{i}}^{t_{i+1}}
[f(t_{i+1},y(t_{i+1}))+\frac{(t-t_{i+1})}{h}
\nabla f(t_{i+1},y(t_{i+1}))+error]dt \\
y_{i+1}-y_i &= &[t f(t_{i+1},y(t_{i+1})) \\
& & +\frac{t(\frac{t}{2}-t_{i+1})}{h}\nabla 
f(t_{i+1},y(t_{i+1}))]_{t_i}^{t_{i+1}}+Error \\
y_{i+1}&=&y(t_i)+ (t_{i+1}-t_i)f(t_{i+1},y(t_{i+1}))\\
& & +\frac{\frac{t_{i+1}^2}{2}-t_{i+1}^2+t_it_{i+1}-\frac{t_i^2}{2}}{h}\nabla(f(t_{i+1},y(t_{i+1}))\\
& & +Error\\
&=&y(t_i)+ hf(t_{i+1},y(t_{i+1}))\\
& & +\frac{-(t_{i+1}-t_i)^2}{2h}(f(t_{i+1},y(t_{i+1}))-f(t_{i},y(t_{i})))\\
& & +Error\\
&=&y(t_i)+ hf(t_{i+1},y(t_{i+1}))\\
& & -\frac{h}{2}(f(t_{i+1},y(t_{i+1}))-f(t_{i},y(t_{i})))+Error\\
&=&y(t_i)+ \frac{h}{2}[f(t_{i+1},y(t_{i+1}))+f(t_{i-1},y(t_{i-1}))]+Error
\end{eqnarray*}
The two step \addtoindex{Adams-Moulton} is $w_0=\alpha_0$ and $w_1=\alpha_1$ with
\[w_{i+1}=w_i+\frac{h}{2}[w_{i+1}+w_{i}] \ \ \ for \ \ i=0,..,N-1 \]

The local truncation error is
\[\tau_{i+1}(h)=\frac{y(t_i+1)-y(t_i)}{h}-\frac{1}{2}[f(t_{i+1},y(t_{i+1}))+f(t_{i},y(t_{i})) ]  \]
\[\tau_{i+1}(h)=\frac{Error}{h}\]

\begin{eqnarray*}
Error &= &\int_{t_i}^{t_{i+1}} \frac{(t-t_{i+1})(t-t_{i})}{2!}f^2(\mu_i,y(\mu_i))]dt \\
&=&\frac{1}{12}h^3f^2(\mu_i,y(\mu_i))\\
\end{eqnarray*}
\[\tau_{i+1}(h)=\frac{\frac{1}{12}h^3f^2(\mu_i,y(\mu_i))}{h}\]
The local truncation error for the one step Adams-Moulton methods is of order 2
\[\tau_{i+1}(h)=O(h^2)\]


\section*{Derivation of the implicit multi-step method (cont)}

As before
\begin{eqnarray*}
y(t_{i+1})-y(t_{i}) &=& \int_{-1}^{0} y^{'}(t_{i+1}+sh) ds\\
&=&
\sum_{k=0}^{m-1}\nabla^k  f(t_{i+1},y(t_{i+1}))h(-1)^k\int_{-1}^{0}\left(\begin{array}{c}-s \\ k \end{array}\right)ds\\
& &+\frac{h^{m+1}}{m!}\int_{-1}^{0}s(s+1)...(s+m-1)f^{m}(\xi,y(\xi))ds.
\end{eqnarray*}
\begin{example}
For k=3 we have 
\begin{eqnarray*}
(-1)^3\int_{-1}^{0}\left(\begin{array}{c}-s \\ k \end{array}\right)ds
&=& \int_{-1}^{0} \frac{-s(-s-1)(-s-2)}{1.2.3}ds\\
&=& \frac{1}{6} \left[ \frac{s^4}{4}+s^3+s^2\right]^{0}_{-1}=-\frac{1}{24}.
\end{eqnarray*}
\end{example}
The general form of the \addtoindex{Adams-Moulton} method is 
\begin{eqnarray*}
y(t_{i+1}) &=&y(t_i)+ h[f(t_{i+1},y(t_{i+1}))-\frac{1}{2}\nabla f(t_{i+1},y(t_{i+1}))-\frac{1}{12}\nabla^2 f(t_{i+1},y(t_{i+1})) - ... ]\\
& & +\frac{h^{m+1}}{m!}\int_{-1}^{0}s(s+1)...(s+m-1)f^{m}(\xi,y(\xi))ds.
\end{eqnarray*}

\section*{Adams-Moulton two step method}
\[ w_0=\alpha, \ \ w_1=\alpha_1,  \]
\[w_{i+1} = w_{i}+\frac{h}{12}[5f(t_{i+1},w_{i+1}) +8 f(t_{i},w_{i})-f(t_{i-1},w_{i-1})] \]
where i=2,3,...,N-1.\\
The local truncation error is 
\[\tau_{i+1}(h) =-\frac{1}{24}h^3 y^4(\mu_i),\]
$\mu_i \in (t_{i-1},t_{i+1}).$

\section*{Adams-Moulton three step method}
\[ w_0=\alpha, \ \ w_1=\alpha_1, \ \ w_2 = \alpha_2, \]
\[w_{i+1} = w_{i}+\frac{h}{24}[9f(t_{i+1},w_{i+1}) +19 f(t_{i},w_{i})-5f(t_{i-1},w_{i-1})+f(t_{i-2},w_{i-2})  ], \]
where i=3,...,N-1.\\
The local truncation error is 
\[\tau_{i+1}(h) =-\frac{19}{720}h^4 y^5(\mu_i),\]
$\mu_i \in (t_{i-2},t_{i+1}).$
\begin{example}
\[ y^{'}=y-t^2+1 \ \ \ 0 \leq t \leq 2 \ \ \ y(0)=0.5 \]
\addtoindex{Adams-Moulton} two step
$w_0=\alpha_0$ and $w_1=\alpha_1$ with
\[w_{i+1}=w_i+\frac{h}{12}[5f(t_{i+1},w_{i+1})+8f(t_{i},w_{i})-f(t_{i-1},w_{i-1})] \] 
\[  for \ \ i=2,..,N-1 \]
truncation error  $ \tau_{i+1}(h)=-\frac{1}{24}h^3 y^4(\mu_i)$ $\mu_i \in (t_{i-1},t_{i+1})$.
\begin{enumerate}
\item Calculate $\alpha_0$ and $\alpha_1$ \\
From the initial condition we have $w_0=0.5$\\
To calculate $w_1$ we use the modified Euler method.
we now have $\alpha_1=w_1=0.826$
\item Calculate $w_i$ for $i=2,...N$
\begin{eqnarray*}
w_{2}&=&w_1+\frac{h}{12}[5f(t_{2},w_{2})\\
& & +8 f(t_{1},w_{1})-f(t_{0},w_{0}) ] \\
&=&w_1+\frac{h}{12}[5(w_{2}+t_2^2+1) \\
& & +8 (w_{1}+t_1^2+1)-(w_{0}+t_0^2+1) ] \\
&=&w_1+\frac{h}{12}[5(w_{2}+t_2^2+1)\\ 
& & +8 (w_{1}+t_1^2+1)-(w_{0}+t_0^2+1) ] \\
.\\
.\\
.\\
(1-\frac{5h}{12})w_{i+1}&=&\frac{h}{12}[[8+\frac{12}{h}]w_{i}-5t_{i+1}^2\\
& & -8t_{i}^2+t_{i-1}^2+12] 
\end{eqnarray*}
\end{enumerate}
\end{example}
This, of course can be generalised.\\
The only unfortunate aspect of the implicit method is that you must convert it into an explicit method, this is not always possible. eg $y^{'}=e^y$.
\section{Table of Adam's methods}
\begin{table}[H]
\centering
\caption{Adams-Bashforth formulas of different order. LTE stands for local truncation error.}
\label{Adams-Bashforth methods}
\begin{tabular}{lllll}
\hline 
Order  &Formula  &LTE   \\
\hline 
 $1$&$y_{n+1}=y_n+hf_{n}$  &$\frac{h^1}{2}y''(\eta)$    \\
 $2$&$y_{n+1}=y_n+\frac{h}{2}[3f_{n}-f_{n-1}] $  &$\frac{5h^2}{12}y'''(\eta)$    \\
 $3$&$y_{n+1}=y_n+\frac{h}{12}[23f_{n}-16f_{n-1}+5f_{n-2}] $  &$\frac{3h^3}{8}y^{(4)}(\eta)$    \\
$4$&$y_{n+1}=y_n+\frac{h}{24}[55f_{n}-59f_{n-1}+37f_{n-2}-9f_{n-3}] $  &$\frac{251h^4}{720}y^{(5)}(\eta)$    \\
 &  &  \\
\hline 
\end{tabular}
\end{table}


\begin{table}[H]
\centering
\caption{Adams-Moulton formulas of different order. LTE stands for local truncation error.}
\label{Adams-Moulton methods}
\begin{tabular}{lllll}
\hline 
Order  &Formula  &LTE   \\
\hline 
 $0$&$y_{n+1}=y_n+hf_{n+1}$  &$-\frac{h^1}{2}y''(\eta)$    \\
 $1$&$y_{n+1}=y_n+\frac{h}{2}[f_{n+1}+f_n] $  &$-\frac{h^2}{12}y'''(\eta)$    \\
 $2$&$y_{n+1}=y_n+\frac{h}{12}[5f_{n+1}+8f_n-f_{n-1}] $  &$-\frac{h^3}{24}y^{(4)}(\eta)$    \\
$3$&$y_{n+1}=y_n+\frac{h}{24}[9f_{n+1}+19f_n-5f_{n-1}+f_{n-2}] $  &$-\frac{19h^5}{720}y^{(4)}(\eta)$    \\
 &  &  \\
\hline 
\end{tabular}
\end{table}

\section{Predictor-Corrector method}
In practice implicit methods are not used as above.  They are used to improve 
approximations obtained by explicit methods. The combination of the two is
called predictor-corrector method.
\begin{example}
Consider the following forth order method for solving an initial-value problem.
\begin{enumerate}
\item
Calculate $w_0,w_1,w_2,w_3$ for the four step \addtoindex{Adams-Bashforth method}, to do this
we use a 4th order one step method, eg Runge Kutta.
\item
Calculate an approximation $w_4$ to $y(t_4)$ using the \addtoindex{Adams-Bashforth method} as
the predictor.
\[w^0_4=w_3+\frac{h}{24}[55f(t_3,w_3)-59f(t_{2},w_{2})+37f(t_1,w_1)-9f(t_0,w_0)] \]
\item
This approximation is improved by inserting $w^0_4$ in the RHS of the three step
\addtoindex{Adams-Moulton} and using it as a corrector
\[w^1_4=w_3+\frac{h}{24}[9f(t_4,w_4^0)+19f(t_{3},w_{3})-5f(t_2,w_2)+f(t_1,w_1)] \]
The only new function evaluation is $f(t_4,w_4^0)$.
\item
$w_4^1$ is the approximation of $y(t_4)$.
\item
Repeat steps 2-4 for calculating the approximation of $y(t_5)$.
\item
Repeat til $y(t_n)$.
\end{enumerate}
\end{example}
Improved approximations to $y(t_{i+1})$ can be obtained by integrating the Adams
Moulton formula
\[w^{k+1}_{i+1}=w_i+\frac{h}{24}[9f(t_{i+1},w_{i+1}^k)+19f(t_{i},w_{i})-5f(t_{i-1},w_{i-1})+f(t_{i-2},w_{i-2})] \]
$w^{k+1}_{i+1}$ converges to the approximation of the implicit method rather than
the solution $y(t_{i+1})$.\\
A more effective method is to reduce step-size if improved accuracy is needed.
\section{Improved step-size multi-step method}
As the predictor corrector technique produces two approximations of each step 
it is a natural candidate for error-control (see previous section).
\begin{example}
The \addtoindex{Adams-Bashforth} 4-step method is the predictor
\[ w_0=\alpha \ \ w_1=\alpha_1 \ \ w_2 = \alpha_2 \ \ w_3=\alpha_3 \]
\begin{eqnarray*}
y(t_{i+1}) &=& y(t_{i})+\frac{h}{24}[55f(t_i,y(t_i)) -59 f(t_{i-1},y(t_{i-1}))\\ 
& & +37f(t_{i-2},y(t_{i-2})) -9 f(t_{i-3},y(t_{i-3}))]\\
& & + \frac{251}{720}h^5 y^5(\mu_i) \end{eqnarray*}
$\mu_i \in (t_{i-3},t_{i+1})$
the truncation error is
\begin{equation}
\label{tunc A}
\frac{y(t_{i+1})-w_{i+1}^0}{h}=\frac{251}{720}h^4 y^5(\mu_i)
\end{equation}
Similarly for \addtoindex{Adams-Moulton} three step method is the corrector
\begin{eqnarray*} y(t_{i+1}) &=& y(t_{i})+\frac{h}{24}[9f(t_{i+1},y(t_{i+1})) +19 f(t_{i},y(t_{i}))\\
& & -5f(t_{i-1},y(t_{i-1})) + f(t_{i-2},y(t_{i-2}))]\\ 
& &-\frac{19}{720}h^5 y^5(\xi_i) \end{eqnarray*}
$\xi_i \in (t_{i-2},t_{i+1})$
the truncation error is
\begin{equation}
\label{tunc B}
\frac{y(t_{i+1})-w_{i+1}}{h}=-\frac{19}{720}h^4 y^5(\xi_i)
\end{equation}
We make the assumption that for small $h$
\[y^5(\xi_i) \approx y^5(\mu_i).\]
Subtracting (\ref{tunc A}) from (\ref{tunc B}) we have
\[\frac{w_{i+1}-w_{i+1}^0}{h}=\frac{h^4}{720}[251y^5(\mu_i)+19y^5(\xi_i)]\approx
\frac{3}{8}h^4y^5(\xi_i), \]
\begin{equation}
y^5(\xi_i) \approx \frac{8}{3h^5}(w_{i+1}-w_{i+1}^0).
\end{equation}
Using this result to eliminate $h^4y^5(\xi_i)$ from (\ref{tunc B})
\[
|\tau_{i+1}(h)| = \frac{|y(t_{i+1})-w_{i+1}|}{h}\approx\frac{19h^4}{720}\frac{8}{3h^5}(|w_{i+1}-w_{i+1}^0|)\]
\[ =\frac{19|w_{i+1}-w_{i+1}^0|}{270h}\]
Now consider a new step size $qh$ generating new approximations $\hat{w}_0,\hat{w}_1,..,\hat{w}_i$
The objective is to choose a q so that the local truncation is bounded by a tol
$\varepsilon$
\[
\frac{|y(t_{i}+qh)-\hat{w}_{i+1}|}{qh}=\frac{19h^4}{720}|y^5(\nu)|q^4\approx\frac{19h^4}{720}\frac{8}{3h^5}(|w_{i+1}-w_{i+1}^0|)q^4
\]
and we need to choose a q so that
\[\frac{|y(t_{i}+qh)-\hat{w}_{i+1}|}{qh}\approx\frac{19q^4|w_{i+1}-w_{i+1}^0|}{270h} < \varepsilon \]
that is, we choose so that
\[ q < \left( \frac{270}{19}\frac{h\varepsilon}{|w_{i+1}-w_{i+1}^0|}\right)^{\frac{1}{4}}\approx 2\left( \frac{h\varepsilon}{|w_{i+1}-w_{i+1}^0|}\right)^{\frac{1}{4}}\]
\end{example}
q is normally chosen as 
\[ q = 1.5\left( \frac{h\varepsilon}{|w_{i+1}-w_{i+1}^0|}\right)^{\frac{1}{4}}\]
With this knowledge we can change step sizes and control out error.

\newpage
\section{Problem Sheet 4 - Multistep Methods}
\begin{enumerate}
\item
Apply the 3-step \addtoindex{Adams-Bashforth} to approximate the solution of the given initial value problems using the indicated number of time steps. Compare the approximate solution with the given exact solution
\begin{enumerate}
\item
$y'=t-y, \ \ (0\leq t \leq 4)$\\
with the initial condition $y(0)=1,$\\
$N=4$, 
$y(t)=2e^{-t}+t-1$\\

\item 
$y'=y-t, \ \ (0\leq t \leq 2)$\\
with the initial condition $y(0)=2,$\\
$N=4$, 
$y(t)=e^{t}+t+1$\\

\end{enumerate}
\item
Apply the 2-step \addtoindex{Adams-Moulton} Method to approximate the solution of the given initial value problems using the indicated number of time steps. Compare the approximate solution with the given exact solution
\begin{enumerate}
\item
$y'=t-y, \ \ (0\leq t \leq 4)$\\
with the initial condition $y(0)=1,$\\
$N=4$, 
$y(t)=2e^{-t}+t-1$\\

\item 
$y'=y-t, \ \ (0\leq t \leq 2)$\\
with the initial condition $y(0)=2,$\\
$N=4$, 
$y(t)=e^{t}+t+1$\\

\end{enumerate}
\item
Derive the difference equation for the 1-step \addtoindex{Adams-Bashforth} method:\\
\[ w_{n+1}=w_n+hf(t_{n},w_{n}),\]
with the local truncation error
\[ \tau_{n+1}(h)=\frac{h}{2}y^{2}(\mu_n)\]
where $\mu_n \in (t_{n},t_{n+1})$.
\item
Derive the difference equation for the 2-step \addtoindex{Adams-Bashforth} method:\\
\[ w_{n+1}=w_n+(\frac{3}{2}hf(t_{n},w_{n})-\frac{1}{2}hf(t_{n-1},w_{n-1})),\]
with the local truncation error
\[ \tau_{n+1}(h)=\frac{5h^2}{12}y^{3}(\mu_n)\]
where $\mu_n \in (t_{n-1},t_{n+1})$.
\item
Derive the difference equation for the 3-step \addtoindex{Adams-Bashforth} method:\\
\[ w_{n+1}=w_n+(\frac{23}{12}hf(t_{n},w_{n})-\frac{4}{3}hf(t_{n-1},w_{n-1})+\frac{5}{12}hf(t_{n-2},w_{n-2})),\]
with the local truncation error
\[ \tau_{n+1}(h)=\frac{9h^3}{24}y^{4}(\mu_n)\]
where $\mu_n \in (t_{n-2},t_{n+1})$.
\item
Derive the difference equation for the 0-step \addtoindex{Adams-Moulton} method:\\
\[ w_{n+1}=w_n+hf(t_{n+1},w_{n+1}),\]
with the local truncation error
\[ \tau_{n+1}(h)=-\frac{h}{2}y^{2}(\mu_n)\]
where $\mu_n \in (t_{n-2},t_{n+1})$.
\item
Derive the difference equation for the 1-step \addtoindex{Adams-Moulton} method:\\
\[ w_{n+1}=w_n+\frac{1}{2}hf(t_{n+1},w_{n+1})+\frac{1}{2}hf(t_{n},w_{n}),\]
with the local truncation error
\[ \tau_{n+1}(h)=-\frac{h^2}{12}y^{3}(\mu_n)\]
where $\mu_n \in (t_{n},t_{n+1})$.
\item
Derive the difference equation for the 2-step \addtoindex{Adams-Moulton} method:\\
\[ w_{n+1}=w_n+\frac{5}{12}hf(t_{n+1},w_{n+1})+\frac{8}{12}hf(t_{n},w_{n})-\frac{1}{12}hf(t_{n-1},w_{n-1}),\]
with the local truncation error
\[ \tau_{n+1}(h)=-\frac{h^3}{24}y^{4}(\mu_n)\]
where $\mu_n \in (t_{n-1},t_{n+1})$.
\item
Derive the difference equation for the 3-step \addtoindex{Adams-Moulton} method:\\
\[ w_{n+1}=w_n+\frac{9}{24}hf(t_{n+1},w_{n+1})+\frac{19}{24}hf(t_{n},w_{n})-\frac{5}{24}hf(t_{n-1},w_{n-1})+\frac{1}{24}hf(t_{n-2},w_{n-2}),\]
with the local truncation error
\[ \tau_{n+1}(h)=-\frac{h^4}{720}y^{5}(\mu_n)\]
where $\mu_n \in (t_{n-2},t_{n+1})$.


\end{enumerate}
\newpage